library/init/meta/interactive.lean
@@ -264,12 +264,7 @@ do e_type ← infer_type e >>= whnf,
    return I
 
 meta def induction (p : parse texpr) (rec_name : parse using_ident) (ids : parse with_ident_list) : tactic unit :=
-do e ← i_to_expr p,
-   match rec_name with
-   | some n := tactic.induction e n ids
-   | none   := do I ← get_type_name e, tactic.induction e (I <.> "rec") ids
-   end,
-   return ()
+do e ← i_to_expr p, tactic.induction e ids rec_name, return ()
 
 meta def cases (p : parse texpr) (ids : parse with_ident_list) : tactic unit :=
 do e ← i_to_expr p,
