tests/lean/induction_tac1.lean
@@ -3,7 +3,7 @@ open tactic
 example (p q : Prop) : p ∨ q → q ∨ p :=
 by do
   H ← intro `H,
-  induction H `or.rec [`Hp, `Hq],
+  induction H [`Hp, `Hq],
   trace_state,
   constructor_idx 2, assumption,
   constructor_idx 1, assumption
@@ -14,7 +14,7 @@ open nat
 example (n : ℕ) : n = 0 ∨ n = succ (pred n) :=
 by do
   n ← get_local `n,
-  induction n `nat.rec [`n', `Hind],
+  induction n [`n', `Hind],
   trace_state,
   constructor_idx 1, reflexivity,
   constructor_idx 2, reflexivity,
@@ -25,7 +25,7 @@ print "-----"
 example (n : ℕ) (H : n ≠ 0) : n > 0 → n = succ (pred n) :=
 by do
   n ← get_local `n,
-  induction n `nat.rec [],
+  induction n [],
   trace_state,
   intro `H1, contradiction,
   intros, reflexivity
